ironfleet/src/Dafny/Distributed/Common/Framework/Performance.s.dfy
@@ -1,0 +1,18 @@
+include "Environment.s.dfy"
+include "Host.s.dfy"
+include "DistributedSystem.s.dfy"
+include "../Collections/Seqs.i.dfy"
+
+module Performance_s {
+  import opened Collections__Seqs_i
+
+  datatype PerformanceReport = None | PerformanceReport(instructions: int, pktsDelivered: int)
+  type PerfReport = PerformanceReport
+
+  predicate {:axiom} PerfLe(lhs:PerfReport, rhs:PerfReport)
+
+  function {:axiom} PerfMax(prs:seq<PerformanceReport>): PerformanceReport
+    ensures forall pr :: pr in prs ==> PerfLe(pr, PerfMax(prs))
+
+  function {:axiom} PerfAdd(pr1:PerformanceReport, pr2:PerformanceReport) : PerformanceReport
+}
